Admitted removed, invariants reworked, Amm postconditions test added

src/Act/Coq.hs
@@ -20,6 +20,7 @@ module Act.Coq where
 import Prelude hiding (GT, LT)
 
 import Data.Map.Strict (Map)
+import Data.Tuple.Extra
 import qualified Data.Map.Strict    as M
 import qualified Data.List.NonEmpty as NE
 import qualified Data.Text          as T
@@ -29,6 +30,7 @@ import Control.Monad.State
 import EVM.ABI
 import Act.Syntax
 import Act.Syntax.TypedExplicit
+import Act.Syntax.Timing (Time(..), Timing(..))
 
 type Fresh = State Int
 
@@ -52,57 +54,53 @@ contractCode store (Contract ctor@Constructor{..} behvs) = T.unlines $
   [ "Module " <> T.pack _cname <> ".\n" ]
   <> [ stateRecord ]
   <> [ base store ctor ]
+  <> [ initPrecs ctor ]
   <> [ postCondConstr ctor ]
   <> [ invariantProps ctor ]
-  <> [ invariants ctor ]
+  <> (concatMap (evalSeq behvConds) (groups behvs))
   <> (concatMap (evalSeq (transition store)) (groups behvs))
-  <> filter ((/=) "") (concatMap (evalSeq retVal) (groups behvs))
+  <> (filter ((/=) "") $ concatMap (evalSeq retVal) (groups behvs))
   <> (concatMap (evalSeq postCondBehv) (groups behvs))
   <> [ step (groups behvs)]
   <> [ initState ctor ]
-  <> [ initArgs ctor ]
   <> [ multistep ]
   <> [ reachable ]
-  <> [ reachableFromInit _cname _cinterface ]
+  <> [ reachableFromInit ctor]
   <> [ invariantInit ctor ]
   <> [ invariantStep ctor ]
-  <> [ reachableInvariant ctor]
+  <> [ invariantReachable ctor]
   <> [ "End " <> T.pack _cname <> "." ]
   where
     groups = groupBy (\b b' -> _name b == _name b')
 
     stateRecord = T.unlines
-      [ "Record " <> stateType <> " : Set := " <> stateConstructor
-      , "{ " <> T.intercalate ("\n" <> "; ") (map decl (M.toList store'))
+
+      [ "Record" <+> stateType <+> ": Set :=" <+> stateConstructor
+      , "{" <+> T.intercalate ("\n" <> "; ") (map decl (M.toList store'))
       , "}."
       ]
 
-    decl (n, (s, _)) = (T.pack n) <> " : " <> slotType s
+    decl (n, (s, _)) = (T.pack n) <+> ":" <+> slotType s
 
     store' = contractStore _cname store
 
 -- | inductive definition of step relation of 2 states
 step :: [[Behaviour]] -> T.Text
 step behvs = inductive
-  stepType "" (stateType <> " -> " <> stateType <> " -> Prop") body
+  stepType "" (stateType <+> "->" <+> stateType <+> "-> Prop") body
   where
     body = concat (evalSeq stepBehv <$> behvs)
 
--- | constructor for the step relation
-stepBehv :: Behaviour -> Fresh T.Text
-stepBehv (Behaviour name _ i _ conds cases _ _ _) =
-  fresh name >>= continuation where
-  continuation name' =
-    return $ name'
-      <> stepSuffix <> " : forall "
-      <> envDecl <> " "
-      <> parens (stateVar <> " : " <> stateType) <> " "
-      <> interface i <> ",\n"
-      <> constructorBody where
-
-    constructorBody = (indent 2) . implication $
-      (coqprop stateVar <$> cases ++ conds)
-      <> [ stepType <+> stateVar <+> parens (name' <+> envVar <+> stateVar <+> arguments i)]
+    -- | constructor for the step relation
+    stepBehv :: Behaviour -> Fresh (T.Text, Maybe T.Text, T.Text)
+    stepBehv (Behaviour name _ i _ _ _ _ _ _) =
+      fresh name >>= continuation where
+      continuation name' =
+        return (name' <> stepSuffix, Just $ envDecl <+> interface i <+> stateDecl, constructorBody)
+        where
+          constructorBody = (indent 2) . implication $
+            [ name' <> "_conds" <+> envVar <+> arguments i <+> stateVar
+            , stepType <+> stateVar <+> parens (name' <+> envVar <+> stateVar <+> arguments i)]
 
 
 -- | definition of reachable states
@@ -110,63 +108,54 @@ reachable :: T.Text
 reachable = definition
   reachableType args value
   where
-    args = parens $ stateVar <> " : " <> stateType
-    value = "exists " <> stateVar' <> ", " <> initStateType <>
-      " " <> stateVar' <> " /\\ " <> multistepType <+>
-      stateVar' <+> stateVar
-    stateVar' = stateVar <> "'"
+    args = parens $ stateVar <+> ":" <+> stateType
+    value = "exists" <+> stateVar' <> "," <+> initStateType <+> stateVar'
+      <+> "/\\" <+> multistepType <+> stateVar' <+> stateVar
 
 -- | specialization of generic multistep
 multistep :: T.Text
 multistep = definition
   multistepType args value
   where
-    args = parens $ stateVar <+> stateVar' <> " : " <> stateType
+    args = parens $ stateVar <+> stateVar' <+> ":" <+> stateType
     value = multistepType <+> stepType <+> stateVar <+> stateVar'
-    stateVar' = stateVar <> "'"
 
--- | definition of reachable states from initial state
-reachableFromInit :: Id -> Interface -> T.Text
-reachableFromInit name i = definition
+-- | definition of reachable states from initial constructor parameters
+reachableFromInit :: Constructor -> T.Text
+reachableFromInit (Constructor name i _ _ _ _ _ ) = definition
   reachableFromInitType args value
   where
     args = envDecl <+> interface i <+> stateDecl
-    value = initArgsType <>
-      " " <> envVar <+> arguments i <> " /\\ " <> multistepType <+>
+    value = initPrecsType <+>
+      envVar <+> arguments i <+> "/\\" <+> multistepType <+>
       parens (T.pack name <+> envVar <+> arguments i) <+> stateVar
 
--- | predicate characterizing all initial (post constructor) states
-initArgs :: Constructor -> T.Text
-initArgs (Constructor _ i@(Interface _ decls) _ conds _ _ _ ) = inductive
-  initArgsType "" (envType <+> interfaceTypes i <+> "Prop") [body]
+-- | definition of constructor preconditions
+initPrecs :: Constructor -> T.Text
+initPrecs (Constructor _ i _ conds _ _ _ ) = definition
+  initPrecsType (envDecl <+> interface i) body
   where
-    body = "InitArgs : " <> universal <> "\n" <> constructorBody
-    --baseval = parens $ T.pack name <+> envVar <+> arguments i
-    constructorBody = (indent 2) . implication . concat $
-      [ coqprop stateVar <$> conds
-      , [initArgsType <+> envVar <+> arguments i]
-      ]
-    universal =
-      "forall " <> envDecl <+>
-      (if null decls
-       then ""
-       else interface i) <> ","
+    body = indent 2 . conjuction . concat $ [coqprop <$> conds]
 
-initState :: Constructor -> T.Text
-initState (Constructor name i@(Interface _ decls) _ conds _ _ _ ) = inductive
-  initStateType "" (stateType <> " -> " <> " Prop") [body]
+-- | definition of behaviour-case conditions
+behvConds :: Behaviour -> Fresh T.Text
+behvConds (Behaviour name _ i _ conds casecs _ _ _) = do
+  name' <- fresh name
+  pure $ definition
+    (name' <> "_conds") (envDecl <+> interface i <+> stateDecl) body
   where
-    body = "InitState : " <> universal <> "\n" <> constructorBody
+    body = (indent 2) (conjuction . concat $ [coqprop <$> (conds <> casecs)])
+
+-- | predicate characterizing all initial (post constructor) states
+initState :: Constructor -> T.Text
+initState (Constructor name i _ _ _ _ _ ) = inductive
+  initStateType "" (stateType <> " -> " <> " Prop") [("InitState", Just $ envDecl <+> interface i, constructorBody)]
+  where
     baseval = parens $ T.pack name <+> envVar <+> arguments i
     constructorBody = (indent 2) . implication . concat $
-      [ coqprop stateVar <$> conds
+      [ [initPrecsType <+> envVar <+> arguments i]
       , [initStateType <+> baseval]
       ]
-    universal =
-      "forall " <> envDecl <+>
-      (if null decls
-       then ""
-       else interface i) <> ","
 
 -- | definition of a base state
 base :: Store -> Constructor -> T.Text
@@ -178,7 +167,7 @@ transition :: Store -> Behaviour -> Fresh T.Text
 transition store (Behaviour name cname i _ _ _ _ rewrites _) = do
   name' <- fresh name
   return $ definition name' (envDecl <+> stateDecl <+> interface i) $
-    stateval store cname (\r _ -> ref stateVar r) rewrites
+    stateval store cname (\r _ -> ref Pre r) rewrites
 
 -- | inductive definition of a return claim
 -- ignores claims that do not specify a return value
@@ -189,142 +178,56 @@ retVal (Behaviour name _ i _ conds cases _ _ (Just r)) =
     (name' <> returnSuffix)
     (envDecl <+> stateDecl <+> interface i)
     (returnType r <> " -> Prop")
-    [retname <> introSuffix <> " :\n" <> body] where
-
+    [(retname <> introSuffix, Nothing, body)] where
 
     retname = name' <> returnSuffix
     body = indent 2 . implication . concat $
-      [ coqprop stateVar <$> conds ++ cases
-      , [retname <+> envVar <+> stateVar <+> arguments i <+> typedexp stateVar r]
+      [ coqprop <$> conds ++ cases
+      , [retname <+> envVar <+> stateVar <+> arguments i <+> typedexp r]
       ]
 
 retVal _ = return ""
 
---postCondConstr :: Constructor -> T.Text
---postCondConstr (Constructor _ _ _ _ [] _ _) = ""
---postCondConstr (Constructor name i _ conds postcs _ _) =
---  lemma
---    (T.pack name <> postSuffix)
---    (envDecl <+> stateDecl <+> interface i)
---    body
---    "Admitted."
---    where
---      body = indent 2 . implication . concat $ 
---        [ --["init STATE"]
---        coqprop "" <$> conds -- state should no be read here so doesn't matter?
---        , ["STATE = " <> T.pack name <+> envVar <+> arguments i]
---        , [T.intercalate " /\\ " $ coqprop stateVar <$> postcs]
---        ]
+-- | Definition of postcondition claim for constructor
 postCondConstr :: Constructor -> T.Text
 postCondConstr (Constructor _ _ _ _ [] _ _) = ""
-postCondConstr (Constructor name i _ conds postcs _ _) =
+postCondConstr (Constructor name i _ _ postcs _ _) =
   T.intercalate "\n\n" $ evalSeq post postcs
     where
-      post :: Exp ABoolean -> Fresh T.Text
-      post pc =
-        fresh (name <> T.unpack postSuffix) >>= continuation where
-        continuation postName = return $
-          lemma
-          postName
-          (envDecl <+> stateDecl <+> interface i)
-          body
-          "Admitted."
-        body = indent 2 . implication . concat $
-          [ --["init STATE"]
-          coqprop "" <$> conds -- state should no be read here so doesn't matter?
-          , ["STATE = " <> T.pack name <+> envVar <+> arguments i]
-          , [coqprop stateVar pc]
+    post :: Exp ABoolean -> Fresh T.Text
+    post pc =
+      fresh (name <> T.unpack postSuffix) >>= continuation where
+      continuation postName = return $ definition postName "" body
+      body = indent 2 $ T.unlines
+        [ forAll $ envDecl <+> interface i <+> stateDecl'
+        , implication . concat $
+          [ [initPrecsType <+> envVar <+> arguments i]
+          , [stateVar' <+> "=" <+> T.pack name <+> envVar <+> arguments i]
+          , [coqprop pc]
           ]
+        ]
 
+-- | Definition of postcondition claim for behaviour cases
 postCondBehv :: Behaviour -> Fresh T.Text
 postCondBehv (Behaviour _ _ _ _ _ _ [] _ _) = return ""
-postCondBehv (Behaviour name _ i _ conds cases postcs _ _) =
+postCondBehv (Behaviour name _ i _ _ _ postcs _ _) =
   fresh name >>= continuation where
   continuation name' = return $ T.intercalate "\n\n" $ evalSeq (post name') postcs
     where
       post :: T.Text -> Exp ABoolean -> Fresh T.Text
       post case_name pc =
         fresh (T.unpack $ case_name <> postSuffix) >>= continuation' where
-        continuation' postName = return $
-          lemma
-          postName
-          (envDecl <+> stateDecl <+> stateDecl' <+> interface i)
-          body
-          "Admitted."
-        body = indent 2 . implication . concat $
-          [ coqprop stateVar <$> conds ++ cases
-          , ["STATE' = " <> name' <+> envVar <+> stateVar <+> arguments i]
-          , [coqprop stateVar pc]
+        continuation' postName = return $ definition postName "" body
+        body = indent 2 $ T.unlines
+          [ forAll $ envDecl <+> stateDecl <+> stateDecl' <+> interface i
+          , implication . concat $
+            [ [name' <> "_conds" <+> envVar <+> arguments i <+> stateVar]
+            , [stateVar' <+> "=" <+> name' <+> envVar <+> stateVar <+> arguments i]
+            , [coqprop pc]
+            ]
           ]
 
-invariantInit :: Constructor -> T.Text
-invariantInit (Constructor name i _ conds _ _ _) =
-  lemma (T.pack name <> invInitSuffix)
-  (envDecl <+> interface i <+> "(P :" <+> envType <+> interfaceTypes i <+> stateType <+> " -> Prop)")
-  claim
-  "Admitted."
-  where
-    claim = indent 2 . implication . concat $
-      [ coqprop "" <$> conds
-      , ["invariant P"]
-      , ["P" <+> envVar <+> arguments i <+> parens (T.pack name <+> envVar <+> arguments i)]
-      ]
--- invariantConstr :: Constructor -> T.Text
--- invariantConstr (Constructor name i _ conds _ invs _) =
---   T.intercalate "\n\n" $ evalSeq inv invs
---   where
---     inv :: Invariant-> Fresh T.Text
---     inv (Invariant _ _ _ (PredTimed p _)) =
---       fresh (name <> T.unpack invInitSuffix) >>= continuation' where
---       continuation' name' = return $
---         lemma
---         name'
---         (envDecl <+> stateDecl <+> interface i)
---         body
---         "Admitted."
---       body = indent 2 . implication . concat $ 
---         [ --["init STATE"]
---         coqprop "" <$> conds -- state should no be read here so doesn't matter?
---         , ["STATE = " <> T.pack name <+> envVar <+> arguments i]
---         , [coqprop stateVar p]
---         ]
-
-invariantStep :: Constructor -> T.Text
-invariantStep (Constructor name i _ conds _ _ _) =
-  lemma (T.pack name <> invStepSuffix)
-  (envDecl <+> interface i <+> stateDecl <+> stateDecl' <+> "(P :" <+> envType <+> interfaceTypes i <+> stateType <+> " -> Prop)")
-  claim
-  "Admitted."
-  where
-    claim = indent 2 . implication . concat $
-      [ coqprop "" <$> conds
-      , ["step" <+> stateVar <+> stateVar <> "'"]
-      , ["invariant P"]
-      , ["P" <+> envVar <+> arguments i <+> stateVar]
-      , ["P" <+> envVar <+> arguments i <+> stateVar <> "'"]
-      ]
-
---invariantStep :: Constructor -> T.Text
---invariantStep (Constructor name i _ conds _ invs _) =
---  T.intercalate "\n\n" $ evalSeq inv invs
---  where
---    inv :: Invariant-> Fresh T.Text
---    inv (Invariant _ _ _ (PredTimed p _)) =
---      fresh (name <> T.unpack invStepSuffix) >>= continuation' where
---      continuation' name' = return $
---        lemma
---        name'
---        (envDecl <+> interface i <+> stateDecl <+> stateDecl')
---        body
---        "Admitted."
---      body = indent 2 . implication . concat $ 
---        [ --["init STATE"]
---          coqprop "" <$> conds -- state should no be read here so doesn't matter?
---        , [stepType <+> stateVar <+> stateVar <> "'"]
---        , [coqprop stateVar p]
---        , [coqprop (stateVar <> "'") p]
---        ]
-
+-- | Definition of invariant propositions
 invariantProps :: Constructor -> T.Text
 invariantProps (Constructor _ i _ _ _ invs _) =
   T.concat $ evalSeq (invariantProp i) invs
@@ -334,22 +237,70 @@ invariantProp i (Invariant _ _ _ (PredTimed p _)) =
   fresh "invariantProp" >>= continuation where
   continuation name' = return $ definition
     name'
-    (envDecl <+> interface i <+> stateDecl)
-    (coqprop stateVar p)
+    (envDecl <+> interface i <+> stateDecl) (coqprop p)
 
-
-invariants :: Constructor -> T.Text
-invariants (Constructor _ i _ _ _ invs _) =
-  inductive
-  "invariant"
-  ""
-  ("(" <> envType <+> interfaceTypes i <+> stateType <> " -> Prop) -> Prop")
-  (evalSeq inv_constructor invs)
+-- | Definition of invariant claim at constructor poststate
+invariantInit :: Constructor -> T.Text
+invariantInit (Constructor name i _ _ _ _ _) =
+  definition invInitType (invPropDecl i) claim
   where
-    inv_constructor :: Invariant -> Fresh T.Text
-    inv_constructor (Invariant _ _ _ (PredTimed _ _)) =
-      fresh' "invariant" "invariantProp" >>= continuation where
-      continuation (constr, term) = return $ constr <> ": invariant " <> term <> "\n"
+    claim = indent 2 $ T.unlines
+      [ forAll $ envDecl <+> interface i
+      , implication . concat $
+        [ [initPrecsType <+> envVar <+> arguments i]
+        , [invPropVar <+> envVar <+> arguments i <+> parens (T.pack name <+> envVar <+> arguments i)]
+        ]
+      ]
+
+-- | Definition of invariant claim for behaviour cases
+invariantStep :: Constructor -> T.Text
+invariantStep (Constructor _ i _ _ _ _ _) =
+  definition invStepType (invPropDecl i) claim
+  where
+    claim = indent 2 $ T.unlines
+      [ forAll $ envDecl <+> interface i <+> stateDecl <+> stateDecl'
+      , implication . concat $
+        [ [initPrecsType <+> envVar <+> arguments i]
+        , [stepType <+> stateVar <+> stateVar']
+        , [invPropVar <+> envVar <+> arguments i <+> stateVar]
+        , [invPropVar <+> envVar <+> arguments i <+> stateVar']
+        ]
+      ]
+
+-- | Lemma extending invariant properties' hold to reachable states,
+-- given proof of init and step invariance
+invariantReachable :: Constructor -> T.Text
+invariantReachable (Constructor _ i _ _ _ _ _) =
+  lemma invReachType "" claim proof
+  where
+    claim = indent 2 $ T.unlines
+      [ forAll (envDecl <+> interface i <+> stateDecl <+> invPropDecl i
+        <+> parens ("HIPinvInit :" <+> invInitType <+> invPropVar) <+> parens ("HPinvStep :" <+> invStepType <+> invPropVar))
+      , implication . concat $
+        [ [reachableFromInitType <+> envVar <+> arguments i <+> stateDecl]
+        , [invPropVar <+> envVar <+> arguments i <+> stateVar]
+        ]
+      ]
+    proof = indent 2 . T.unlines $
+      [
+       "Proof.",
+       "intros" <+> envVar <+> arguments i <+> stateVar <+> invPropVar <+> "HIPinvInit HIPinvStep Hreach.",
+       "unfold reachableFromInit in Hreach.",
+       "destruct Hreach as [Hinit Hmulti].",
+       "apply step_multi_step with (P := fun s s' =>" <+> invPropVar <+> envVar <+> arguments i <+> "s ->" <+> invPropVar <+> envVar <+> arguments i <+> "s' ) in Hmulti.",
+       "- apply Hmulti.",
+       "  apply HIPinvInit; assumption.",
+       "- intros s s' Hstep.",
+       "  apply HIPinvStep with (STATE := s) (STATE' := s') ; assumption.",
+       "- unfold Relation_Definitions.reflexive.",
+       "  intros.",
+       "  assumption.",
+       "- unfold Relation_Definitions.transitive.",
+       "  intros s1 s2 s3 Ht1 Ht2 Ht3.",
+       "  apply Ht2, Ht1.",
+       "  assumption.",
+       "Qed."
+     ]
 
 -- | produce a state value from a list of storage updates
 -- 'handler' defines what to do in cases where a given name isn't updated
@@ -386,7 +337,7 @@ updateVar store updates handler focus t@(StorageValue (ContractType cid)) =
     -- Only some fields are updated
     ([], updates'@(_:_)) -> parens $ T.unwords $ (T.pack cid <> "." <> stateConstructor) : fmap (\(n, (t', _)) -> updateVar store  updates' handler (focus' n) t') (M.toList store')
     -- No fields are updated, whole contract may be updated with some call to the constructor
-    (updates', []) -> foldl (\ _ (Update _ _ e) -> coqexp stateVar e) (handler focus t) updates'
+    (updates', []) -> foldl (\ _ (Update _ _ e) -> coqexp e) (handler focus t) updates'
     -- The contract is updated with constructor call and field accessing. Unsupported.
     (_:_, _:_) -> error "Cannot handle multiple updates to contract variable"
   where
@@ -400,31 +351,31 @@ updateVar _ updates handler focus t@(StorageValue (PrimitiveType _)) =
   foldl updatedVal (handler focus t) (filter (eqRef focus) updates)
     where
       updatedVal _ (Update SByteStr _ _) = error "bytestrings not supported"
-      updatedVal _ (Update _ _ e) = coqexp stateVar e
+      updatedVal _ (Update _ _ e) = coqexp e
 
 updateVar _ updates handler focus t@(StorageMapping xs _) = parens $
-  lambda n <> foldl updatedMap prestate (filter (baseRef focus) updates)
+  lambda n <+> foldl updatedMap prestate (filter (baseRef focus) updates)
     where
       prestate = parens $ handler focus t <+> lambdaArgs n
       n = length xs
 
       updatedMap _ (Update SByteStr _ _) = error "bytestrings not supported"
       updatedMap prestate' (Update _ item e) =
-        let ixs = ixsFromItem item in -- This will not work if the domain is a contract type
-        "if " <> boolScope (T.intercalate " && " (map cond (zip ixs ([0..] :: [Int]))))
-        <> " then " <> coqexp stateVar e
-        <> " else " <> prestate'
+        let ixs = ixsFromItem item in
+        "if" <+> boolScope (T.intercalate " && " (map cond (zip ixs ([0..] :: [Int]))))
+        <+> "then" <+> coqexp e
+        <+> "else" <+> prestate'
 
-      cond (TExp argType _ arg, i) = parens $ anon <> T.pack (show i) <> eqsym argType <> coqexp stateVar arg
+      cond (TExp argType _ arg, i) = parens $ anon <> T.pack (show i) <> eqsym argType <> coqexp arg
 
-      lambda i = if i >= 0 then "fun " <> lambdaArgs i <> " => " else ""
+      lambda i = if i >= 0 then "fun" <+> lambdaArgs i <+> "=>" else ""
 
       lambdaArgs i = T.unwords $ map (\a -> anon <> T.pack (show a)) ([0..i-1] :: [Int])
 
       eqsym :: SType a -> T.Text
       eqsym argType = case argType of
-        SInteger -> " =? "
-        SBoolean -> " =?? "
+        SInteger -> "=?"
+        SBoolean -> "=??"
         SByteStr -> error "bytestrings not supported"
         SSArray _ -> error "arrays not supported"
 
@@ -433,15 +384,11 @@ updateVar _ updates handler focus t@(StorageMapping xs _) = parens $
 interface :: Interface -> T.Text
 interface (Interface _ decls) =
   T.unwords $ map decl decls where
-  decl (Decl t name) = parens $ T.pack name <> " : " <> abiType t
+  decl (Decl t name) = parens $ T.pack name <+> ":" <+> abiType t
 
 arguments :: Interface -> T.Text
 arguments (Interface _ decls) =
   T.unwords $ map (\(Decl _ name) -> T.pack name) decls
-
-interfaceTypes :: Interface -> T.Text
-interfaceTypes (Interface _ decls) =
-  T.pack "->" <> T.intercalate " -> " (map (\(Decl t _) -> abiType t) decls) <> (if decls == [] then "" else T.pack " -> ")
 
 -- | coq syntax for a slot type
 slotType :: SlotType -> T.Text
@@ -472,10 +419,10 @@ returnType (TExp (SSArray _) _ _) = error "arrays not supported"
 -- this is used in cases where a value is not set in the constructor
 defaultSlotValue :: SlotType -> T.Text
 defaultSlotValue (StorageMapping xs t) = parens $
-  "fun "
-  <> T.unwords (replicate (length (NE.toList xs)) "_")
-  <> " => "
-  <> defaultVal t
+  "fun"
+  <+> T.unwords (replicate (length (NE.toList xs)) "_")
+  <+> "=>"
+  <+> defaultVal t
 defaultSlotValue (StorageValue t) = defaultVal t
 
 defaultVal :: ValueType -> T.Text
@@ -490,101 +437,99 @@ abiVal AbiStringType = strMod <> ".EmptyString"
 abiVal _ = error "TODO: missing default values"
 
 -- | coq syntax for an expression
-coqexp :: T.Text -> Exp a -> T.Text
+coqexp :: Exp a -> T.Text
 -- booleans
-coqexp _ (LitBool _ True)  = "true"
-coqexp _ (LitBool _ False) = "false"
-coqexp s (And _ e1 e2)  = parens $ "andb "   <> coqexp s e1 <+> coqexp s e2
-coqexp s (Or _ e1 e2)   = parens $ "orb"     <> coqexp s e1 <+> coqexp s e2
-coqexp s (Impl _ e1 e2) = parens $ "implb"   <> coqexp s e1 <+> coqexp s e2
-coqexp s (Eq _ _ e1 e2)   = parens $ coqexp s e1  <> " =? " <> coqexp s e2
-coqexp s (NEq _ _ e1 e2)  = parens $ "negb " <> parens (coqexp s e1  <> " =? " <> coqexp s e2)
-coqexp s (Neg _ e)      = parens $ "negb " <> coqexp s e
-coqexp s (LT _ e1 e2)   = parens $ coqexp s e1 <> " <? "  <> coqexp s e2
-coqexp s (LEQ _ e1 e2)  = parens $ coqexp s e1 <> " <=? " <> coqexp s e2
-coqexp s (GT _ e1 e2)   = parens $ coqexp s e2 <> " <? "  <> coqexp s e1
-coqexp s (GEQ _ e1 e2)  = parens $ coqexp s e2 <> " <=? " <> coqexp s e1
+coqexp (LitBool _ True)  = "true"
+coqexp (LitBool _ False) = "false"
+coqexp (And _ e1 e2)  = parens $ "andb"    <+> coqexp e1 <+> coqexp e2
+coqexp (Or _ e1 e2)   = parens $ "orb"     <+> coqexp e1 <+> coqexp e2
+coqexp (Impl _ e1 e2) = parens $ "implb"   <+> coqexp e1 <+> coqexp e2
+coqexp (Eq _ _ e1 e2)   = parens $ coqexp e1  <+> "=?" <+> coqexp e2
+coqexp (NEq _ _ e1 e2)  = parens $ "negb" <+> parens (coqexp e1  <+> "=?" <+> coqexp e2)
+coqexp (Neg _ e)      = parens $ "negb" <+> coqexp e
+coqexp (LT _ e1 e2)   = parens $ coqexp e1 <+> "<?"  <+> coqexp e2
+coqexp (LEQ _ e1 e2)  = parens $ coqexp e1 <+> "<=?" <+> coqexp e2
+coqexp (GT _ e1 e2)   = parens $ coqexp e2 <+> "<?"  <+> coqexp e1
+coqexp (GEQ _ e1 e2)  = parens $ coqexp e2 <+> "<=?" <+> coqexp e1
 
 -- integers
-coqexp _ (LitInt _ i) = T.pack $ show i
-coqexp s (Add _ e1 e2) = parens $ coqexp s e1 <> " + " <> coqexp s e2
-coqexp s (Sub _ e1 e2) = parens $ coqexp s e1 <> " - " <> coqexp s e2
-coqexp s (Mul _ e1 e2) = parens $ coqexp s e1 <> " * " <> coqexp s e2
-coqexp s (Div _ e1 e2) = parens $ coqexp s e1 <> " / " <> coqexp s e2
-coqexp s (Mod _ e1 e2) = parens $ "Z.modulo " <> coqexp s e1 <> coqexp s e2
-coqexp s (Exp _ e1 e2) = parens $ coqexp s e1 <> " ^ " <> coqexp s e2
-coqexp _ (IntMin _ n)  = parens $ "INT_MIN "  <> T.pack (show n)
-coqexp _ (IntMax _ n)  = parens $ "INT_MAX "  <> T.pack (show n)
-coqexp _ (UIntMin _ n) = parens $ "UINT_MIN " <> T.pack (show n)
-coqexp _ (UIntMax _ n) = parens $ "UINT_MAX " <> T.pack (show n)
+coqexp (LitInt _ i) = T.pack $ show i
+coqexp (Add _ e1 e2) = parens $ coqexp e1 <+> "+" <+> coqexp e2
+coqexp (Sub _ e1 e2) = parens $ coqexp e1 <+> "-" <+> coqexp e2
+coqexp (Mul _ e1 e2) = parens $ coqexp e1 <+> "*" <+> coqexp e2
+coqexp (Div _ e1 e2) = parens $ coqexp e1 <+> "/" <+> coqexp e2
+coqexp (Mod _ e1 e2) = parens $ "Z.modulo" <+> coqexp e1 <+> coqexp e2
+coqexp (Exp _ e1 e2) = parens $ coqexp e1 <+> "^" <+> coqexp e2
+coqexp (IntMin _ n)  = parens $ "INT_MIN"  <+> T.pack (show n)
+coqexp (IntMax _ n)  = parens $ "INT_MAX"  <+> T.pack (show n)
+coqexp (UIntMin _ n) = parens $ "UINT_MIN" <+> T.pack (show n)
+coqexp (UIntMax _ n) = parens $ "UINT_MAX" <+> T.pack (show n)
 
-coqexp s (InRange _ t e) = coqexp s (bound t e)
+coqexp (InRange _ t e) = coqexp (bound t e)
 
 -- polymorphic
-coqexp s (VarRef _ _ _ e) = entry s e
-coqexp s (ITE _ b e1 e2) = parens $ "if "
-                               <> coqexp s b
-                               <> " then "
-                               <> coqexp s e1
-                               <> " else "
-                               <> coqexp s e2
+coqexp (VarRef _ whn _ e) = entry whn e
+coqexp (ITE _ b e1 e2) = parens $ "if"
+                               <+> coqexp b
+                               <+> "then"
+                               <+> coqexp e1
+                               <+> "else"
+                               <+> coqexp e2
 
 -- environment values
 -- Relies on the assumption that Coq record fields have the same name
 -- as the corresponding Haskell constructor
-coqexp _ (IntEnv _ envVal) = parens $ T.pack (show envVal) <+> envVar
+coqexp (IntEnv _ envVal) = parens $ T.pack (show envVal) <+> envVar
 -- Contracts
-coqexp s (Create _ cid args) = parens $ T.pack cid <> "." <> T.pack cid <+> envVar <+> coqargs s args
+coqexp (Create _ cid args) = parens $ T.pack cid <> "." <> T.pack cid <+> envVar <+> coqargs args
 -- unsupported
-coqexp _ Cat {} = error "bytestrings not supported"
-coqexp _ Slice {} = error "bytestrings not supported"
-coqexp _ ByStr {} = error "bytestrings not supported"
-coqexp _ ByLit {} = error "bytestrings not supported"
-coqexp _ ByEnv {} = error "bytestrings not supported"
-coqexp _ Array {} = error "arrays not supported"
+coqexp Cat {} = error "bytestrings not supported"
+coqexp Slice {} = error "bytestrings not supported"
+coqexp ByStr {} = error "bytestrings not supported"
+coqexp ByLit {} = error "bytestrings not supported"
+coqexp ByEnv {} = error "bytestrings not supported"
+coqexp Array {} = error "arrays not supported"
 
 -- | coq syntax for a proposition
-coqprop :: T.Text -> Exp a -> T.Text
-coqprop _ (LitBool _ True)  = "True"
-coqprop _ (LitBool _ False) = "False"
-coqprop s (And _ e1 e2)  = parens $ coqprop s e1 <> " /\\ " <> coqprop s e2
-coqprop s (Or _ e1 e2)   = parens $ coqprop s e1 <> " \\/ " <> coqprop s e2
-coqprop s (Impl _ e1 e2) = parens $ coqprop s e1 <> " -> " <> coqprop s e2
-coqprop s (Neg _ e)      = parens $ "not " <> coqprop s e
-coqprop s (Eq _ _ e1 e2)   = parens $ coqexp s e1 <> " = "  <> coqexp s e2
-coqprop s (NEq _ _ e1 e2)  = parens $ coqexp s e1 <> " <> " <> coqexp s e2
-coqprop s (LT _ e1 e2)   = parens $ coqexp s e1 <> " < "  <> coqexp s e2
-coqprop s (LEQ _ e1 e2)  = parens $ coqexp s e1 <> " <= " <> coqexp s e2
-coqprop s (GT _ e1 e2)   = parens $ coqexp s e1 <> " > "  <> coqexp s e2
-coqprop s (GEQ _ e1 e2)  = parens $ coqexp s e1 <> " >= " <> coqexp s e2
-coqprop s (InRange _ t e) = coqprop s (bound t e)
+coqprop :: Exp a -> T.Text
+coqprop (LitBool _ True)  = "True"
+coqprop (LitBool _ False) = "False"
+coqprop (And _ e1 e2)  = parens $ coqprop e1 <+> "/\\" <+> coqprop e2
+coqprop (Or _ e1 e2)   = parens $ coqprop e1 <+> "\\/" <+> coqprop e2
+coqprop (Impl _ e1 e2) = parens $ coqprop e1 <+> "->"  <+> coqprop e2
+coqprop (Neg _ e)      = parens $ "not" <+> coqprop e
+coqprop (Eq _ _ e1 e2)   = parens $ coqexp e1 <+> "="  <+> coqexp e2
+coqprop (NEq _ _ e1 e2)  = parens $ coqexp e1 <+> "<>" <+> coqexp e2
+coqprop (LT _ e1 e2)   = parens $ coqexp e1 <+> "<"  <+> coqexp e2
+coqprop (LEQ _ e1 e2)  = parens $ coqexp e1 <+> "<=" <+> coqexp e2
+coqprop (GT _ e1 e2)   = parens $ coqexp e1 <+> ">"  <+> coqexp e2
+coqprop (GEQ _ e1 e2)  = parens $ coqexp e1 <+> ">=" <+> coqexp e2
+coqprop (InRange _ t e) = coqprop (bound t e)
 
-coqprop _ e = error "ill formed proposition: " <> T.pack (show e)
+coqprop e = error "ill formed proposition:" <+> T.pack (show e)
 
 -- | coq syntax for a typed expression
-typedexp :: T.Text -> TypedExp -> T.Text
-typedexp s (TExp _ _ e) = coqexp s e
+typedexp :: TypedExp -> T.Text
+typedexp (TExp _ _ e) = coqexp e
 
-entry :: T.Text -> TItem k a -> T.Text
+entry :: Time 'Timed -> TItem k a -> T.Text
 entry _ (Item SByteStr _ _) = error "bytestrings not supported"
-entry s (Item _ _ r) = ref s r
+entry whn (Item _ _ r) = ref whn r
 
-ref :: T.Text -> Ref k -> T.Text
-ref s (SVar _ _ name) = parens $ T.pack name <+> s
+ref :: Time 'Timed -> Ref k -> T.Text
+ref Pre (SVar _ _ name) = parens $ T.pack name <+> stateVar
+ref Post (SVar _ _ name) = parens $ T.pack name <+> stateVar'
 ref _ (CVar _ _ name) = T.pack name
-ref s (SArray _ r _ ixs) = parens $ ref s r <+> coqargs s (fst <$> ixs)
-ref s (SMapping _ r _ ixs) = parens $ ref s r <+> coqargs s ixs
-ref s (SField _ r cid name) = parens $ T.pack cid <> "." <> T.pack name <+> ref s r
+ref whn (SArray _ r _ ixs) = parens $ ref whn r <+> coqargs (fst <$> ixs)
+ref whn (SMapping _ r _ ixs) = parens $ ref whn r <+> coqargs ixs
+ref whn (SField _ r cid name) = parens $ T.pack cid <> "." <> T.pack name <+> ref whn r
 
 -- | coq syntax for a list of arguments
-coqargs :: T.Text -> [TypedExp] -> T.Text
-coqargs s es = T.unwords (map (typedexp s) es)
+coqargs :: [TypedExp] -> T.Text
+coqargs es = T.unwords (map typedexp es)
 
 fresh :: Id -> Fresh T.Text
 fresh name = state $ \s -> (T.pack (name <> show s), s + 1)
-
-fresh' :: Id -> Id -> Fresh (T.Text, T.Text)
-fresh' constr term = state $ \s -> ((T.pack (constr <> show s), T.pack (term <> show s)), s + 1)
 
 evalSeq :: Traversable t => (a -> Fresh b) -> t a -> t b
 evalSeq f xs = evalState (sequence (f <$> xs)) 0
@@ -593,62 +538,42 @@ evalSeq f xs = evalState (sequence (f <$> xs)) 0
 
 definition :: T.Text -> T.Text -> T.Text -> T.Text
 definition name args value = T.unlines
-  [ "Definition " <> name <+> args <> " :="
+  [ "Definition" <+> name <+> args <+> ":="
   , value <> "."
   ]
 
-inductive :: T.Text -> T.Text -> T.Text -> [T.Text] -> T.Text
+inductive :: T.Text -> T.Text -> T.Text -> [(T.Text, Maybe T.Text, T.Text)] -> T.Text
 inductive name args indices constructors = T.unlines
-  [ "Inductive " <> name <+> args <> " : " <> indices <> " :="
-  , (T.concat $ ("| " <>) <$> constructors) <> "."
+  [ "Inductive" <+> name <+> args <+> ":" <+> indices <+> ":="
+  , T.unlines (((<>) "| " . uncurry3 inductiveConstructor) <$> constructors) <> "."
   ]
+
+inductiveConstructor :: T.Text -> Maybe T.Text -> T.Text -> T.Text
+inductiveConstructor ctorName Nothing body =
+     ctorName <+> ":\n" <> body
+inductiveConstructor ctorName (Just bindings) body =
+     ctorName <+> ":" <+> forAll bindings <> "\n" <> body
 
 lemma :: T.Text -> T.Text -> T.Text -> T.Text -> T.Text
 lemma name args claim proof = T.unlines
-  [ "Lemma " <> name <+> args <> " : "
+  [ "Lemma" <+> name <+> args <+> ":"
   , claim <> "."
   , proof
   ]
 
-reachableInvariant :: Constructor -> T.Text
-reachableInvariant (Constructor name i _ _ _ _ _) =
-  lemma "inv_reach"
-  ""
-  --(envDecl <+> interface i <+> stateDecl <+> "(P :" <+> envType <+> interfaceTypes i <+> stateType <+> " -> Prop)")
-  claim
-  proof
-  where
-    claim = indent 2 . implication . concat $
-      [ ["forall" <+> (envDecl <+> interface i <+> stateDecl <+> "(P :" <+> envType <+> interfaceTypes i <+> stateType <+> " -> Prop)") <> ",\nreachableFromInit " <+> envVar <+> arguments i <+> stateDecl]
-      , ["invariant P"]
-      , ["P" <+> envVar <+> arguments i <+> stateVar]
-      ]
-    proof = indent 2 . T.unlines $
-      [
-       "Proof.",
-       "intros" <+> envVar <+> arguments i <+> stateVar <+> "P Hreach HinvP.",
-       "unfold reachableFromInit in Hreach.",
-       "destruct Hreach as [Hinit Hmulti].",
-       "destruct Hinit.",
-       "apply step_multi_step with (P := fun s s' => P" <+> envVar <+> arguments i <+> "s  -> P" <+> envVar <+> arguments i <+> "s' ) in Hmulti.",
-       "- apply Hmulti.",
-       "apply" <+> T.pack name <> "_invInit; assumption.",
-       "- intros s s' Hstep.",
-       "apply" <+> T.pack name <> "_invStep with (STATE := s) (STATE' := s') ; assumption.",
-       "- unfold Relation_Definitions.reflexive.",
-       "intros.",
-       "assumption.",
-       "- unfold Relation_Definitions.transitive.",
-       "intros s1 s2 s3 Ht1 Ht2 Ht3.",
-       "apply Ht2, Ht1.",
-       "assumption.",
-       "Qed."
-     ]
--- "Theorem inv_reach :\n forall (ENV : Env) (STATE : State) " <> "(P :" <+> envType <+> interfaceTypes i <+> stateType <+> " -> Prop)" <> ",\n reachableFromInit ("<> name <> " ENV) STATE\n -> invariant P\n -> P ENV STATE.\n Proof.\n intros ENV STATE P Hreach HinvP.\n unfold reachableFromInit in Hreach.\n destruct Hreach as [Hinit Hmulti].\n apply step_multi_step with (P := fun s s' => P ENV s  -> P ENV s' ) in Hmulti.\n - apply Hmulti.\n apply "<> name <>"_invInit.\n + assumption.\n - intros s s' Hstep.\n apply " <> name <> "_invStep with (STATE := s) (STATE' := s') ; assumption.\n - unfold Relation_Definitions.reflexive.\n intros.\n assumption.\n - unfold Relation_Definitions.transitive.\n intros s1 s2 s3 Ht1 Ht2 Ht3.\n apply Ht2, Ht1.\n assumption.\n Qed."
+
+-- | forall bindings
+forAll :: T.Text -> T.Text
+forAll bindings = "forall" <+> bindings <> ","
 
 -- | multiline implication
 implication :: [T.Text] -> T.Text
 implication xs = "   " <> T.intercalate "\n-> " xs
+
+-- | multiline conjuction
+conjuction :: [T.Text] -> T.Text
+conjuction [] = "   True"
+conjuction xs = "   " <> T.intercalate "\n/\\ " xs
 
 -- | wrap text in parentheses
 parens :: T.Text -> T.Text
@@ -659,6 +584,11 @@ boolScope s = "(" <> s <> ")%bool"
 
 indent :: Int -> T.Text -> T.Text
 indent n = T.unlines . fmap (T.replicate n " " <>) . T.lines
+
+(<+>) :: T.Text -> T.Text -> T.Text
+"" <+> t2 = t2
+t1 <+> "" = t1
+t1 <+> t2 = t1 <> " " <> t2
 
 --- constants ---
 
@@ -676,14 +606,17 @@ stateType = "State"
 stateVar :: T.Text
 stateVar = "STATE"
 
+stateVar' :: T.Text
+stateVar' = "STATE'"
+
 nextVar :: T.Text
 nextVar = "NEXT"
 
 stateDecl :: T.Text
-stateDecl = parens $ stateVar <> " : " <> stateType
+stateDecl = parens $ stateVar <+> ":" <+> stateType
 
 stateDecl' :: T.Text
-stateDecl' = parens $ stateVar <> "' : " <> stateType
+stateDecl' = parens $ stateVar' <+> ":" <+> stateType
 
 stateConstructor :: T.Text
 stateConstructor = "state"
@@ -694,11 +627,14 @@ returnSuffix = "_ret"
 postSuffix :: T.Text
 postSuffix = "_post"
 
-invInitSuffix :: T.Text
-invInitSuffix  = "_invInit"
+invInitType :: T.Text
+invInitType  = "invariantInit"
 
-invStepSuffix :: T.Text
-invStepSuffix  = "_invStep"
+invStepType :: T.Text
+invStepType  = "invariantStep"
+
+invReachType :: T.Text
+invReachType  = "invariantReachable"
 
 baseSuffix :: T.Text
 baseSuffix = "_base"
@@ -715,8 +651,20 @@ stepType = "step"
 initStateType :: T.Text
 initStateType = "init"
 
-initArgsType :: T.Text
-initArgsType = "initArgs"
+invPropVar :: T.Text
+invPropVar = "IP"
+
+invPropType :: Interface -> T.Text
+invPropType (Interface _ decls) = T.intercalate " -> " $ concat [[envType], map (\(Decl t _) -> abiType t) decls, [stateType, "Prop"]]
+
+invPropDecl :: Interface -> T.Text
+invPropDecl i = parens $ invPropVar <+> ":" <+> invPropType i
+
+initPrecsType :: T.Text
+initPrecsType = "initPreconds"
+
+behvPrecsType :: T.Text
+behvPrecsType = "behvPrecs"
 
 multistepType :: T.Text
 multistepType = "multistep"
@@ -737,11 +685,7 @@ envVar :: T.Text
 envVar = "ENV"
 
 envDecl :: T.Text
-envDecl = parens $ envVar <> " : " <> envType
+envDecl = parens $ envVar <+> ":" <+> envType
 
 anon :: T.Text
 anon = "_binding_"
-
-(<+>) :: T.Text -> T.Text -> T.Text
-t1 <+> t2 = t1 <> " " <> t2
-
