Makefile
@@ -60,7 +60,7 @@ hevm_multi_fast=$(filter-out $(hevm_multi_slow), $(hevm_multi_pass))
 failing_typing=tests/frontend/pass/dss/vat.act tests/frontend/pass/creation/createMultiple.act tests/frontend/pass/staticstore/staticstore.act
 
 
-coq-examples = tests/coq/transitions tests/coq/safemath tests/coq/exponent tests/coq/token tests/coq/ERC20-simple tests/coq/ERC20 tests/coq/multi
+coq-examples = tests/coq/transitions tests/coq/safemath tests/coq/exponent tests/coq/token tests/coq/ERC20-simple tests/coq/ERC20 tests/coq/multi tests/coq/amm
 
 .PHONY: test-coq $(coq-examples)
 test-coq: compiler $(coq-examples)
